HelloTypeSystem/Util.lean
@@ -4,3 +4,19 @@ theorem Nat.add_same {n : _root_.Nat} : n + n = 2 * n :=
   calc
     _ = 1 * n + 1 * n := by rw [Nat.one_mul]
     _ = _             := Nat.add_mul 1 1 _ |> .symm
+
+def Set (α : Type u) := α → Prop
+instance : EmptyCollection (Set α) where
+  emptyCollection := fun _ => False
+instance : Singleton α (Set α) where
+  singleton x := fun y => x = y
+instance : Membership α (Set α) where
+  mem x s := s x
+instance : Union (Set α) where
+  union a b := fun x => x ∈ a ∨ x ∈ b
+instance : SDiff (Set α) where
+  sdiff a b := fun x => x ∈ a ∧ ¬ x ∈ b
+instance : HasSubset (Set α) where
+  Subset a b := ∀ x ∈ a, x ∈ b
+
+theorem singleton_mem_uniq {a x : α} : a ∈ ({ x } : Set α) → x = a := id
